lean/dk_math/DkMath/Collatz/PetalBridge.lean
@@ -20,6 +20,7 @@ import DkMath.Collatz.PetalBridge.PressureDecay
 import DkMath.Collatz.PetalBridge.PressureFrontier
 import DkMath.Collatz.PetalBridge.PressureAccounting
 import DkMath.Collatz.PetalBridge.OneCycle
+import DkMath.Collatz.PetalBridge.ValuationFlowBridge
 import DkMath.Collatz.PetalBridge.Collision
 
 #print "file: DkMath.Collatz.PetalBridge"
